libs/ffi/FFICallbacks.mli
@@ -1,6 +1,12 @@
 type callbacks = int64
 
 val ocaml_ticket_cb: callbacks -> callbacks -> string -> string -> string -> unit
+
+val ocaml_cert_select_cb: callbacks -> callbacks -> string -> string -> (callbacks * int) option
+val ocaml_cert_format_cb: callbacks -> callbacks -> callbacks -> string
+val ocaml_cert_sign_cb: callbacks -> callbacks -> callbacks -> int -> string -> string option
+val ocaml_cert_verify_cb: callbacks -> callbacks -> string -> int -> string*string -> bool
+
 val ocaml_send_tcp: callbacks -> string -> Z.t
 val ocaml_recv_tcp: callbacks -> string -> Z.t
 
