src/pki/mipki.c
@@ -1,0 +1,510 @@
+/* -------------------------------------------------------------------- */
+#include <sys/types.h>
+#include <sys/stat.h>
+#include <stdlib.h>
+#include <stdint.h>
+#include <string.h>
+#include <assert.h>
+#include <time.h>
+
+#include <openssl/err.h>
+#include <openssl/pem.h>
+#include <openssl/x509v3.h>
+
+#include "mipki.h"
+
+// The parsed representation of chains and private keys
+typedef struct {
+  X509* endpoint;
+  STACK_OF(X509) *intermediates;
+  EVP_PKEY* key;
+  int is_universal;
+} config_entry;
+
+/********************** GLOBAL VARIABLES ***********************/
+// We cache the loading of certificate chains and private keys
+// They remain in memory until mipki_cleanup() is called
+X509_STORE *g_store;
+config_entry *g_config;
+size_t g_config_len;
+
+
+/*
+          rsa_pkcs1_sha1(0x0201),
+          rsa_pkcs1_sha256(0x0401),
+          rsa_pkcs1_sha384(0x0501),
+          rsa_pkcs1_sha512(0x0601),
+          ecdsa_sha1(0x0203),
+
+          ecdsa_secp256r1_sha256(0x0403),
+          ecdsa_secp384r1_sha384(0x0503),
+          ecdsa_secp521r1_sha512(0x0603),
+
+          rsa_pss_sha256(0x0804),
+          rsa_pss_sha384(0x0805),
+          rsa_pss_sha512(0x0806),
+
+          ed25519(0x0807),
+          ed448(0x0808),
+
+          obsolete_RESERVED(0x0000..0x0200),
+          dsa_sha1_RESERVED(0x0202),
+          obsolete_RESERVED(0x0204..0x0400),
+          dsa_sha256_RESERVED(0x0402),
+          obsolete_RESERVED(0x0404..0x0500),
+          dsa_sha384_RESERVED(0x0502),
+          obsolete_RESERVED(0x0504..0x0600),
+          dsa_sha512_RESERVED(0x0602),
+          obsolete_RESERVED(0x0604..0x06FF),
+          private_use(0xFE00..0xFFFF),
+          (0xFFFF)
+      } SignatureScheme;
+*/
+
+// Debugging function to inspect certificates loaded by the store
+static int cert_verify_cb(int ok, X509_STORE_CTX *ctx)
+{
+#ifdef DEBUG
+    char buf[512];
+    static int cb_index = 0;
+
+    printf("Starting cb #%d (ok = %d)\n", ++cb_index, ok);
+    if(X509_STORE_CTX_get_error(ctx) == X509_V_OK) {
+      printf("Callback reports no error.\n");
+    } else {
+      printf("Error string = '%s'\n",
+        X509_verify_cert_error_string(X509_STORE_CTX_get_error(ctx)));
+    }
+
+    X509 *cur = X509_STORE_CTX_get0_cert(ctx);
+    X509_NAME_oneline(X509_get_subject_name(cur), buf, 256);
+    printf("current_cert subject:   %s\n",buf);
+    X509_NAME_oneline(X509_get_issuer_name(cur), buf, 256);
+    printf("current_cert issuer:    %s\n",buf);
+#endif
+
+    return ok;
+}
+
+typedef struct {
+  password_callback cb;
+  const char *info;
+} pass_cb_state;
+
+int password_cb(char *buf, int size, int rwflag, void *p)
+{
+  pass_cb_state *s = (pass_cb_state*)p;
+  return s->cb(buf, size, s->info);
+}
+
+void mipki_cleanup()
+{
+  for(size_t i=0; i<g_config_len; i++)
+  {
+    config_entry *cfg = g_config + i;
+    X509_free(cfg->endpoint);
+    EVP_PKEY_free(cfg->key);
+    sk_X509_pop_free(cfg->intermediates, X509_free);
+  }
+
+  free(g_config);
+  X509_STORE_free(g_store);
+  OPENSSL_thread_stop();
+}
+
+int mipki_init(const mipki_config_entry config[], size_t config_len, password_callback pcb, int *erridx)
+{
+  *erridx = -1;
+  if(!OPENSSL_init_crypto(OPENSSL_INIT_LOAD_CRYPTO_STRINGS, NULL))
+    return 0;
+
+  g_store = X509_STORE_new();
+  if(!g_store) return 0;
+
+  if(!X509_STORE_set_default_paths(g_store)) return 0;
+  X509_STORE_set_verify_cb_func(g_store, cert_verify_cb);
+
+  g_config = malloc(sizeof(config_entry) * config_len);
+  if(!g_config) return 0;
+  g_config_len = 0;
+
+  for(size_t i = 0; i < config_len; i++)
+  {
+    *erridx = i;
+    config_entry *cfg = g_config + i;
+    const mipki_config_entry *cur = config + i;
+    pass_cb_state cbs = {.cb = pcb, .info = cur->key_file};
+
+    STACK_OF(X509) *chain = sk_X509_new_null();
+    X509 *x509 = NULL;
+
+    if(!chain) return 0;
+
+    BIO *bio = BIO_new_file(cur->key_file, "r");
+    if(!bio) return 0;
+
+    EVP_PKEY* sk = PEM_read_bio_PrivateKey(bio, NULL, password_cb, (void*)&cbs);
+    if(!sk || !BIO_free(bio)) return 0;
+
+    bio = BIO_new_file(cur->cert_file, "r");
+    if(!bio) return 0;
+
+    for(size_t j = 0; ; j++)
+    {
+      x509 = PEM_read_bio_X509_AUX(bio, NULL, NULL, NULL);
+
+      if(!x509) {
+        int n = ERR_peek_last_error();
+
+        if(!j || !(ERR_GET_LIB(n) == ERR_LIB_PEM && ERR_GET_REASON(n) == PEM_R_NO_START_LINE))
+          return 0;
+        else
+          break; // Chain is complete, allegedly
+      }
+
+      // Check that the private key matches the first certificate in the file
+      if(!j) {
+        if(!X509_check_private_key(x509, sk))
+          return 0;
+
+        cfg->endpoint = x509;
+      } else {
+        sk_X509_push(chain, x509);
+      }
+    }
+
+    cfg->intermediates = chain;
+    cfg->is_universal = cur->is_universal;
+  }
+
+  return 1;
+}
+
+int mipki_add_root_file_or_path(const char *ca_file)
+{
+  struct stat sb;
+
+  if(!stat(ca_file, &sb))
+    return 0;
+
+  if(S_ISDIR(sb.st_mode))
+    return X509_STORE_load_locations(g_store, NULL, ca_file);
+
+  return X509_STORE_load_locations(g_store, ca_file, NULL);
+}
+
+void* mipki_select_certificate(const char *sni, mipki_signature *algs, size_t algs_len, mipki_signature *selected)
+{
+  for(size_t i = 0; i < g_config_len; i++)
+  {
+    config_entry *cfg = g_config + i;
+    char *peername = NULL;
+
+    // Server-side hostname validation to match wildcards, SAN, etc
+    if(cfg->is_universal || X509_check_host(cfg->endpoint, sni, strlen(sni), 0, &peername))
+    {
+      if(peername) printf("Found matching entry in certificate names: %s\n", peername);
+      int curve, kt = EVP_PKEY_base_id(cfg->key);
+      *selected = 0;
+
+      for(size_t j = 0; j < algs_len; j++)
+      {
+        mipki_signature alg = algs[i];
+        uint8_t low = algs[j] & 0xFF;
+        uint8_t high = algs[j] >> 8;
+
+        switch(kt)
+        {
+          case EVP_PKEY_RSA:
+            if((high == 8 && (low == 4 || low == 5 || low == 6)) ||
+               (low == 1 && high >= 2 && high <= 6))
+              *selected = alg;
+            break;
+
+          case EVP_PKEY_ED25519:
+            if(high == 8 && low == 7)
+              *selected = alg;
+            break;
+
+          case EVP_PKEY_EC:
+            curve = EC_GROUP_get_curve_name(EC_KEY_get0_group(EVP_PKEY_get0_EC_KEY(cfg->key)));
+            if((curve == NID_X9_62_prime256v1 && high == 4 && low == 3) ||
+               (curve == NID_secp384r1 && high == 5 && low == 3) ||
+               (curve == NID_secp521r1 && high == 6 && low == 3) ||
+               (high == 2 && low == 3))
+              *selected = alg;
+            break;
+        }
+
+        if(*selected) return (void*)cfg;
+      }
+    }
+  }
+
+  *selected = 0;
+  return NULL;
+}
+
+/*
+int EVP_DigestSignInit(EVP_MD_CTX *ctx, EVP_PKEY_CTX **pctx,
+                       const EVP_MD *type, ENGINE *e, EVP_PKEY *pkey);
+int EVP_DigestSignUpdate(EVP_MD_CTX *ctx, const void *d, size_t cnt);
+int EVP_DigestSignFinal(EVP_MD_CTX *ctx, unsigned char *sig, size_t *siglen);
+*/
+
+static const EVP_MD *sha(int variant) {
+    switch (variant) {
+      case 0: return EVP_sha1();
+      case 1: return EVP_sha256();
+      case 2: return EVP_sha384();
+      case 3: return EVP_sha512();
+    }
+    return NULL;
+}
+
+size_t mipki_sign(const void *cert_ptr, const mipki_signature sigalg, const char *tbs, size_t tbs_len, char *sig)
+{
+  config_entry *cfg = (config_entry*)cert_ptr;
+  EVP_MD_CTX *ctx = EVP_MD_CTX_new();
+  const EVP_MD *md;
+  EVP_PKEY_CTX* key_ctx = EVP_PKEY_CTX_new(cfg->key, NULL);
+  return 0;
+/*
+  if(EVP_DigestSignInit(md_ctx, key_ctx, md, NULL, cfg->key) != 1)
+
+  switch(sigalg)
+  {
+    case 0x0804: // rsa_pss_sha256
+    case 0x0805: // rsa_pss_sha384
+    case 0x0806: // rsa_pss_sha512
+      md = sha(sigalg - 0x0803);
+      break;
+  }
+
+  if(pss == Val_true) {
+
+      caml_failwith("openssl_stub: EVP_PKEY_CTX_set_rsa_padding PSS");
+    if(EVP_PKEY_CTX_set_rsa_pss_saltlen(key_ctx, RSA_PSS_SALTLEN_DIGEST) != 1)
+      caml_failwith("openssl_stub: EVP_PKEY_CTX_set_rsa_pss_saltlen");
+  } else {
+    if (EVP_PKEY_CTX_set_rsa_padding(key_ctx, RSA_PKCS1_PADDING) != 1)
+      caml_failwith("openssl_stub: EVP_PKEY_CTX_set_rsa_padding PKCS1");
+  }
+
+  if(EVP_DigestSign(md_ctx, (uint8_t*)String_val(output), &olen,
+      (uint8_t*) String_val(data), caml_string_length(data)) != 1) {
+#ifdef DEBUG
+    printf("ocaml_rsa_sign: caml_string_length(data)=%zu, RSA_size(rsa)=%u\n",
+      caml_string_length(data), RSA_size(rsa));
+#endif
+    unsigned long err = ERR_peek_last_error();
+    char* err_string = ERR_error_string(err, NULL);
+    caml_failwith(err_string);
+  }
+  */
+}
+
+/*
+static void* get_key(X509* x509, key_type *type)
+{
+  *type = key_unknown;
+  EVP_PKEY* pk = X509_get_pubkey(x509);
+  if(!pk) return NULL;
+
+  switch(EVP_PKEY_base_id(pk))
+  {
+    case EVP_PKEY_RSA:
+      RSA* rsa = EVP_PKEY_get1_RSA(pk);
+      *type = key_rsa;
+      return (void*)rsa;
+
+    case EVP_PKEY_DSA:
+      DSA* dsa = EVP_PKEY_get1_DSA(pk);
+      *type = key_dsa;
+      return (void*)dsa;
+      if (!dsa) CAMLreturn(Val_none);
+      (void) DSA_set_method(dsa, DSA_OpenSSL());
+      DSA_val(mldsa) = dsa;
+      mlkey = caml_alloc(1, 1); // CertDSA
+      Store_field(mlkey, 0, mldsa);
+      break;
+
+    case EVP_PKEY_EC:
+      mlec = caml_alloc_custom(&key_ops, sizeof(EC_KEY*), 0, 1);
+      EC_KEY* eck = EVP_PKEY_get1_EC_KEY(pk);
+      break;
+
+    default:
+      CAMLreturn(Val_none);
+  }
+}*/
+
+/*
+size_t ocaml_ecdsa_sign(EC_KEY *key, const char *data, size_t data_len, char *output)
+{
+  size_t olen;
+  if (ECDSA_sign(0, data, data_len, output, &olen, key) == 0) {
+    return 0;
+  }
+  return olen;
+}
+
+int ocaml_ecdsa_verify(EC_KEY *key, const char *data, size_t data_len, const char *sig, size_t sig_len)
+{
+  return ECDSA_verify(0, data, data_len, sig, sig_len, key) > 0;
+}
+*/
+
+/*
+CAMLprim value ocaml_validate_chain(value chain, value for_signing, value hostname, value cafile) {
+    CAMLparam4(chain, for_signing, hostname, cafile);
+
+    time_t current_time;
+    STACK_OF(X509) *sk;
+    sk = sk_X509_new_null();
+    X509* top_cert = NULL;
+    char *host;
+
+    if(chain == Val_emptylist) CAMLreturn(Val_false);
+    if(hostname == Val_none) host = NULL;
+    else host = String_val(Some_val(hostname));
+
+    do {
+      value head = Field(chain, 0);
+      size_t len = caml_string_length(head);
+      X509* x509;
+      unsigned char *cert = (unsigned char*)String_val(head);
+      x509 = d2i_X509(NULL, (const unsigned char**) &cert, len);
+//      printf("ADDING CERT[%d]\n", (int)len);
+      if(!top_cert) top_cert = x509; else sk_X509_push(sk, x509);
+      chain = Field(chain, 1);
+    }
+    while(chain != Val_emptylist);
+
+    X509_STORE_CTX *ctx = NULL;
+    X509_STORE *store = NULL;
+    X509_VERIFY_PARAM *param = NULL;
+
+    current_time = time(NULL);
+    store = X509_STORE_new();
+    ctx = X509_STORE_CTX_new();
+    param = X509_VERIFY_PARAM_new();
+    if(!ctx || !store || !param) CAMLreturn(Val_false);
+
+    // Validation parameters
+    X509_VERIFY_PARAM_set_flags(param, X509_V_FLAG_USE_CHECK_TIME | X509_V_FLAG_CRL_CHECK_ALL);
+    X509_VERIFY_PARAM_set_time(param, current_time);
+    X509_VERIFY_PARAM_set1_host(param, host, 0);
+    X509_STORE_set1_param(store, param);
+
+    X509_STORE_CTX_init(ctx, store, top_cert, sk);
+
+    int r = X509_verify_cert(ctx);
+//    printf("X509_verify_cert() == %d [%s]\n", r, X509_verify_cert_error_string(ctx->error));
+
+    X509_STORE_free(store);
+    X509_STORE_CTX_free(ctx);
+    sk_X509_free(sk);
+    X509_VERIFY_PARAM_free(param);
+
+    CAMLreturn(r==1 ? Val_true : Val_false);
+}
+
+CAMLprim value ocaml_load_chain(value pem) {
+  CAMLparam1(pem);
+
+  char *pemfile = (char*)String_val(pem);
+  BIO *bio = BIO_new_file(pemfile, "r");
+  if(!bio) CAMLreturn(Val_none);
+
+  int c = 0;
+  unsigned long n = 0;
+  X509 *x509, *first = NULL;
+
+  CAMLlocal2(mlc, mlret);
+  mlret = Val_emptylist;
+
+  ERR_clear_error();
+
+  // Try to read all x509 structs in the file
+  do {
+    x509 = PEM_read_bio_X509_AUX(bio, NULL, NULL, NULL);
+
+    if(!c) first = x509;
+
+    if(!x509)
+    {
+      n = ERR_peek_last_error();
+      if(!c ||
+	 !(ERR_GET_LIB(n) == ERR_LIB_PEM
+	  && ERR_GET_REASON(n) == PEM_R_NO_START_LINE))
+	CAMLreturn(Val_none);
+      else break;
+    }
+
+    int len;
+    unsigned char *buf = NULL;
+    len = i2d_X509(x509, &buf);
+    if (len < 0) CAMLreturn(Val_none); // Yes there is a leak there
+
+    CAMLlocal1(der_cert);
+    der_cert = caml_alloc_string(len);
+    memcpy(String_val(der_cert), buf, len);
+
+    mlc = caml_alloc(2, 0);
+    Store_field(mlc, 0, der_cert);
+    Store_field(mlc, 1, mlret);
+    mlret = mlc;
+  }
+  while(++c);
+
+  CAMLreturn(Val_some(mlret));
+}
+
+CAMLprim value ocaml_load_key(value pem) {
+  CAMLparam1(pem);
+
+  char *pemfile = (char*)String_val(pem);
+  BIO *bio = BIO_new_file(pemfile, "r");
+  if(!bio) CAMLreturn(Val_none);
+
+
+  if(!sk) CAMLreturn(Val_none);
+  CAMLlocal4(mlkey, mlrsa, mldsa, mlec);
+
+  switch(EVP_PKEY_base_id(sk))
+  {
+    case EVP_PKEY_RSA:
+      mlrsa = caml_alloc_custom(&evp_rsa_ops, sizeof(RSA*), 0, 1);
+      RSA* rsa = EVP_PKEY_get1_RSA(sk);
+      if(!rsa) CAMLreturn(Val_none);
+      RSA_val(mlrsa) = rsa;
+      mlkey = caml_alloc(1, 0); // CertRSA
+      Store_field(mlkey, 0, mlrsa);
+      break;
+
+    case EVP_PKEY_DSA:
+      mldsa = caml_alloc_custom(&evp_dsa_ops, sizeof(DSA*), 0, 1);
+      DSA* dsa = EVP_PKEY_get1_DSA(sk);
+      if (!dsa) CAMLreturn(Val_none);
+      DSA_val(mldsa) = dsa;
+      mlkey = caml_alloc(1, 1); // CertDSA
+      Store_field(mlkey, 0, mldsa);
+      break;
+
+    case EVP_PKEY_EC:
+      mlec = caml_alloc_custom(&key_ops, sizeof(EC_KEY*), 0, 1);
+      EC_KEY* eck = EVP_PKEY_get1_EC_KEY(sk);
+      if(!eck) CAMLreturn(Val_none);
+      EC_KEY_val(mlec) = eck;
+      mlkey = caml_alloc(1, 2); // CertECDSA
+      Store_field(mlkey, 0, mlec);
+      break;
+
+    default:
+      CAMLreturn(Val_none);
+  }
+
+  CAMLreturn(Val_some(mlkey));
+}
+*/
