src/pki/mipki.h
@@ -1,0 +1,21 @@
+#ifndef HEADER_MIPKIH
+#define HEADER_MIPKIH
+#include <stdint.h>
+
+typedef struct {
+  const char *cert_file;
+  const char *key_file;
+  int is_universal;
+} mipki_config_entry;
+
+typedef uint16_t mipki_signature;
+
+// A callback used to ask for the passphrase of the private key
+typedef int (*password_callback)(char *pass, int max_size, const char *key_file);
+
+int mipki_init(const mipki_config_entry config[], size_t config_len, password_callback pcb, int *erridx);
+int mipki_add_root_file_or_path(const char *ca_file);
+void* mipki_select_certificate(const char *sni, mipki_signature *algs, size_t algs_len, mipki_signature *selected);
+size_t mipki_sign(const void *cert_ptr, const mipki_signature sigalg, const char *tbs, size_t tbs_len, char *sig);
+
+#endif
