src/pki/test.c
@@ -1,0 +1,23 @@
+#include <stdio.h>
+#include <stdint.h>
+#include "mipki.h"
+
+int main(int argc, char **argv)
+{
+  mipki_config_entry config[1] = {
+    {
+      .cert_file = "../../data/server.crt",
+      .key_file = "../../data/server.key",
+      .is_universal = 0
+    }
+  };
+  int erridx;
+
+  if(!mipki_init(config, 1, NULL, &erridx))
+  {
+    printf("FAILURE: errid=%d\n", erridx);
+    return 1;
+  }
+  printf("INIT OK\n");
+  return 0;
+}
